# 2.1 Linear Equation

## Solve first order linear DE

1. First please make sure the equation MUST start with the form below.

$$
\frac{d y}{d t}+p(t) y=g(t) \tag{1}
$$

Where $p(t)$ and $g(t)$ are continuous functions. 



2. Then we assume there is a function $\mu(t)$, which is **integrating factor**. and let integrating factor multiply everything in (1).

$$
\mu(t) \frac{d y}{d t}+\mu(t) p(t) y=\mu(t) g(t) \tag{2}
$$

3. Assume $\mu(t)$ satisfy

$$
\mu(t) p(t)=\mu^{\prime}(t)
$$

Then plug it back to rquation (2), then we will get 
$$
\mu(t) \frac{d y}{d t}+\mu^{\prime}(t) y=\mu(t) g(t) \tag{3}
$$


4. We can knoe that the equation in left hand side of (3) is product rule. $\mu(t) \frac{d y}{d t}+\mu^{\prime}(t) y=(\mu(t) y(t))^{\prime}$. Then we can have a new equation.

$$
(\mu(t) y(t))^{\prime}=\mu(t) g(t) \tag{4}
$$



5. Now we need to integrate both sides

$$
\begin{gathered}
\int(\mu(t) y(t))^{\prime} d t=\int \mu(t) g(t) d t \\
\mu(t) y(t)+c=\int \mu(t) g(t) d t
\end{gathered}
$$

6. Then the final step will be.

$$
\begin{aligned}
\mu(t) y(t) &=\int \mu(t) g(t) d t-c \\
y(t) &=\frac{\int \mu(t) g(t) d t-c}{\mu(t)}
\end{aligned}
$$

No matter $-c$ or $+c$, since $c$ is constant. 



## What is $\mu$ in the equation?

1. We know 

$$
\mu(t) p(t)=\mu^{\prime}(t)
$$

2. Divide both side by $\mu(t)$. 

$$
\frac{\mu^{\prime}(t)}{\mu(t)}=p(t)
$$

and we can simplify it to 
$$
(\ln \mu(t))^{\prime}=p(t)
$$


3. then we can integrate both sides to get. 

$$
\begin{aligned}
\ln \mu(t)+k &=\int p(t) d t \\
\ln \mu(t) &=\int p(t) d t+k
\end{aligned}
$$

4. Exponentiate bothe sides to get $\mu(t)$ out of the natural logarithm.

$$
\begin{aligned}
\mu(t) &=\mathbf{e}^{\int p(t) d t+k} \\
&=\mathbf{e}^k \mathbf{e}^{\int p(t) d t}
\end{aligned}
$$

Again, since $e^k$ is constant we can just write as $k$. 
$$
\mu(t)=k \mathbf{e}^{\int p(t) d t}
$$




## Example

![](https://github.com/WilliamYKZ/Picture/raw/main/JPEG%20image-C7297E918D2C-1.jpeg)